\documentclass[class=article, crop=false]{standalone}
\input{../preamble.tex}


\fancyhf{}
\lhead{Nathan Solomon}
\rhead{Page \thepage}
\pagestyle{fancy}

\begin{document}
\section{4/12/2024 lecture}

\subsection{Group actions}
A \emph{(left) group action} (of a group $G$ on a set $M$) is a map $\cdot: G \times M \rightarrow M$ which is
\begin{enumerate}
    \item Unital, meaning $e \cdot m = m$ for any $M \in M$, and
    \item Associative, meaning $(gh)\cdot m = g \cdot (h \cdot m)$ for any $g \in G, m \in M$.
\end{enumerate}
For any group $G$, there is an obvious (left) group action of $G$ on itself, given by (left) multiplication.

GET NOTES ON LEFT/RIGHT GROUP ACTION, CAYLEY'S THEOREM, ORBITS (define conjugacy classes as orbits of the conjugation action), STABILIZER SUBGROUP, CENTER, DIHEDRAL GROUP, ORBIT-STABILIZER THEOREM, etc.

\subsection{Dihedral group}
We can define the action of this group on the elements of the $xy$-plane in terms of reflections and rotations. ALSO GIVE GROUP PRESENTATION
\begin{note}
    W use $D_n$ to mean the set of symmetries of a regular $n$-gon, which is a group with $2n$ elements, but some people use $D_{2n}$ to mean that same group.
\end{note}

\subsection{Orbit-stabilizer theorem}
\begin{thm}
    If $G$ acts on $M$, then
    \[ \abs{G \cdot m} \times \abs{G_m} = \abs{G} \]
    for any $m \in M$.
    \par
    If $G$ acts on $M$ via a right group action instead of a left group action, then replace $G \cdot m$ with $m \cdot G$.
\end{thm}
\begin{proof}
    Let $f: G/G_m \rightarrow G \cdot m$ be a homomorphism defined by $f(gG_m) = g \cdot m$. This is well-defined because for any two representative elements $gG_m$ and $ghG_m$ of $G/G_m$,
    \[ f(gG_m)=g\cdot m = g \cdot (h \cdot m) = (gh) \cdot m = f(ghG_m). \]
    Also, $f$ is surjective because every element of the orbit has the form $g \cdot m$. It's injective because if $g \cdot m = g' \cdot m$, then
    \[ \left( g' \right)^{-1} \cdot (g \cdot m) = \left( g' \right)^{-1} \cdot (g' \cdot m) = m, \]
    which implies $ \left( g' \right)^{-1} g \in G_m$, so $gG_m=g'G_m$.
\end{proof}

\begin{prop}
    Let $C(g)$ be the conjugacy class of some element $g$ of a group. If that group is $S_n$, then $C(g)$ can also be denoted as $C(a_1,\dots,a_n)$, where $a_i$ is the number of $i$-cycles in $g$. Then
    \[ \abs{C(a_1,\dots,a_n)} = \frac{n!}{\prod_{j=1}^n j^{a_j} \left( a_j! \right) }. \]
    INCLUDE PROOF OF THIS
\end{prop}

\subsection{Fixed point theorem}
Let $G$ be a finite group acting on a set $M$ such that for any $g \in G, g \neq e$, only finitely many $m$ are fixed by $g$.
\par
Let $Y = \left\{ (m,g): g \neq e, g \cdot m = m \right\}$. Then
\[ \sum_{g \neq e} \abs{ \left\{ m\in M:g \cdot m=m \right\}} = \abs{Y} = \sum_{m \in M} \left( \abs{G_m}-1 \right) . \]
This is also equal to
\[ \sum_\text{orbits} \abs{ \frac{G}{G_m}} \left( \abs{G_m}-1 \right) . \]
where $m$ is any element of the orbit.
\begin{cor}
    If $G$ is a finite subgroup of $SO(3)$ which acts on the unit sphere $M=S^2$, then
    \[ 2 \left( 1 - \frac{1}{n} \right) = r - \sum{i=1}^r \frac{1}{n_i}, \]
    where $r$ is the number of group orbits of ???
    FINISH THIS PROOF AND EXPLAIN INTUITION FOR IT
\end{cor}

\end{document}
